Common.lean
@@ -10,7 +10,4 @@ import Common.Parsing
 import Common.Nat
 import Common.Substring
 import Common.BitVec
-import Common.Finite
-import Common.Countable
-import Common.HashSet
 import Common.Function
