Common/Countable.lean
@@ -1,9 +1,0 @@
-import Common.Finite
-
-class Countable (α : Type u) where
-  enumerate : α → Nat
-  injective {a b : α} : enumerate a = enumerate b → a = b
-
-instance {α : Type u} [Finite α] : Countable α where
-  enumerate := Fin.val ∘ Finite.enumerate
-  injective :=  Finite.injective ∘ Fin.val_inj.mp
